proof/refine/CSpace1_R.thy
@@ -1,0 +1,16 @@
+(*
+ * Copyright 2014, General Dynamics C4 Systems
+ * Copyright 2020, Data61, CSIRO (ABN 41 687 119 230)
+ * Copyright 2023, Proofcraft Pty Ltd
+ *
+ * SPDX-License-Identifier: GPL-2.0-only
+ *)
+
+(* CSpace refinement *)
+
+theory CSpace1_R
+imports
+  ArchCSpace_I
+begin
+
+end
